Some progress on AFInd for ctrees

theories/CTree/Logic/AF.v
@@ -40,7 +40,9 @@ Section BasicLemmas.
       eapply done_not_ktrans with (t:=t); eauto.
   Qed.
 
-  (* This lemma is crucial but forces us to have enumerable branches *)
+  (* This lemma forces us to have finite branches.
+     Alternatively, a classical φ would also allow
+     us to work without induction on branch arity. *)
   Lemma af_brD_aux: forall n (k: fin' n -> ctree E X) w φ,
       (forall (i: fin' n), <( {k i}, w |= AF now φ )>) -> 
       φ w \/ (forall i, can_step (k i) w /\
@@ -49,15 +51,13 @@ Section BasicLemmas.
   Proof.
     induction n; intros.
     - specialize (H Fin.F1).
-      next in H.
-      destruct H.
+      next in H; destruct H.
       + now left.
       + right.
         intro i.
-        dependent destruction i.
-        * next in H.
-          destruct H; intuition.
-        * dependent destruction i.
+        dependent destruction i; try solve [inv i].
+        next in H.
+        destruct H; intuition.
     - (* Need to construct [k, i] *)
       pose proof (H Fin.F1).
       edestruct IHn with (k:=fun (i: fin (S n)) =>
@@ -135,206 +135,215 @@ Section BasicLemmas.
 End BasicLemmas.
 
 Section AfIndLemma.
-  Context {E: Type} {HE: Encode E} {X: Type}
-    (φ: ctree E X -> World E -> Prop).
-  
-  (*| [t |= AF φ] is semantic and requires double induction, on [AF] and inside it, in
-  [ktrans]. Attempt to simplify to one induction with [AFInd] |*)
-  Inductive AFInd: ctree E X -> World E -> Prop :=
-  | AFIndBase: forall (t: ctree E X) (w: World E),
-      φ t w ->
-      AFInd t w
-  | AFIndDoneBase: forall t (x: X),
+  Context {E: Type} {HE: Encode E} {X: Type}.
+
+  (* t, w |= WF now φ *)
+  Inductive AFNowInd(φ: World E -> Prop): ctree E X -> World E -> Prop :=
+  | AFNowIndBase: forall (t: ctree E X) (w: World E),
+      φ w ->
+      AFNowInd φ t w
+  | AFNowIndDone: forall t (x: X),
       observe t = RetF x ->
-      φ Ctree.stuck (Done x) ->
-      AFInd t Pure
-  | AFIndFinishBase: forall t (e: E) (v: encode e) (x: X),
+      φ (Done x) ->
+      AFNowInd φ t Pure
+  | AFNowIndFinish: forall t (e: E) (v: encode e) (x: X),
       observe t = RetF x ->
-      φ Ctree.stuck (Finish e v x) ->
-      AFInd t (Obs e v)
-  | AFIndBr: forall t w b n (k: fin' n -> ctree E X),
+      φ (Finish e v x) ->
+      AFNowInd φ t (Obs e v)
+  | AFNowIndBr: forall t w b n (k: fin' n -> ctree E X),
       observe t = BrF b n k ->
-      (forall (i: fin' n), AFInd (k i) w) ->
-      AFInd t w
-  |AFIndVis: forall (t: ctree E X) w e k (_: encode e),
+      not_done w ->
+      (forall (i: fin' n), can_step (k i) w -> AFNowInd φ (k i) w) ->
+      AFNowInd φ t w
+  | AFNowIndVis: forall (t: ctree E X) w e k,
       observe t = VisF e k ->
       not_done w ->
-      (forall (v: encode e), AFInd (k v) (Obs e v)) ->
-      AFInd t w.
+      (forall (v: encode e), AFNowInd φ (k v) (Obs e v)) ->
+      AFNowInd φ t w.
 
-  Global Instance proper_equ_afind {HP: Proper (equ eq ==> eq ==> iff) φ}:
-    Proper (equ eq ==> eq ==> iff) AFInd.
+  Global Instance proper_equ_afind φ:
+    Proper (equ eq ==> eq ==> iff) (AFNowInd φ).
   Proof.
     unfold Proper, respectful.
     intros; subst; split; intros Hind.
     - generalize dependent y.
       induction Hind; intros.
-      + apply AFIndBase; auto.
-        now rewrite <- H0.
-      + apply AFIndDoneBase with x; auto.
-        unfold equ in H1; step in H1; cbn in H1; dependent destruction H1; congruence.
-      + apply AFIndFinishBase with x; auto.
-        unfold equ in H1; step in H1; cbn in H1; dependent destruction H1; congruence.
-      + step in H2; cbn in H2; rewrite H in H2.
-        dependent destruction H2.
-        eapply AFIndBr with b n k2; auto.
-        intro i.
-        eapply H1, H2.
+      + apply AFNowIndBase; auto.
+      + apply AFNowIndDone with x; auto.
+        unfold equ in H1; step in H1; cbn in H1;
+          dependent destruction H1; congruence.
+      + apply AFNowIndFinish with x; auto.
+        unfold equ in H1; step in H1; cbn in H1;
+          dependent destruction H1; congruence.
       + step in H3; cbn in H3; rewrite H in H3.
         dependent destruction H3.
-        eapply AFIndVis with e k2; auto.
+        eapply AFNowIndBr with b n k2; auto.
+        intros i (t' & w' & TR').
+        eapply H2 with i; [|apply H3].
+        assert (Heqi: k i ≅ k2 i) by apply H3; auto.
+        rewrite Heqi. 
+        now (exists t', w').
+      + step in H3; cbn in H3; rewrite H in H3.
+        dependent destruction H3.
+        eapply AFNowIndVis with e k2; auto.
         intros.
         apply H2, H3.
     - generalize dependent x.
       induction Hind; intros.
-      + apply AFIndBase; auto.
-        now rewrite H0.
-      + apply AFIndDoneBase with x; auto.
-        unfold equ in H1; step in H1; cbn in H1; dependent destruction H1; congruence.
-      + apply AFIndFinishBase with x; auto.
-        unfold equ in H1; step in H1; cbn in H1; dependent destruction H1; congruence.
-      + step in H2; cbn in H2; rewrite H in H2.
-        dependent destruction H2.
-        eapply AFIndBr with b n k1; auto.
-        intro i.
-        eapply H1, H2.
+      + apply AFNowIndBase; auto.        
+      + apply AFNowIndDone with x; auto.
+        unfold equ in H1; step in H1; cbn in H1;
+          dependent destruction H1; congruence.
+      + apply AFNowIndFinish with x; auto.
+        unfold equ in H1; step in H1; cbn in H1;
+          dependent destruction H1; congruence.
       + step in H3; cbn in H3; rewrite H in H3.
         dependent destruction H3.
-        eapply AFIndVis with e k1; auto.
+        eapply AFNowIndBr with b n k1; auto.
+        intros i (t' & w' & TR').
+        assert (Heqi: k1 i ≅ k i) by apply H3; auto.
+        eapply H2 with i; auto.
+        rewrite <- Heqi.
+        now (exists t', w').
+      + step in H3; cbn in H3; rewrite H in H3.
+        dependent destruction H3.
+        eapply AFNowIndVis with e k1; auto.
         intros.
         apply H2, H3.
-  Qed.      
-
-  Lemma af_ind_stuck_done: forall (x: X),
-    AFInd Ctree.stuck (Done x) <->
-    φ Ctree.stuck (Done x).
-  Proof.
-    split; intros.
-    - Transparent Ctree.stuck. dependent induction H; auto.
-      cbn in x0; dependent destruction x0.
-      apply H1; eauto.
-      exact Fin.F1.
-    - now apply AFIndBase.
   Qed.
 
-  Lemma af_ind_stuck_finish: forall (e: E) (v: encode e) (x: X),
-    AFInd Ctree.stuck (Finish e v x) <->
-    φ Ctree.stuck (Finish e v x).
+  Lemma afind_brD_aux: forall n (k: fin' n -> ctree E X) w φ,
+      (forall i, AFNowInd φ (k i) w) ->
+      φ w \/ (forall i, can_step (k i) w /\
+                    (forall t' w', [k i, w] ↦ [t', w'] ->
+                              AFNowInd φ t' w')).
   Proof.
-    split; intros.
-    - dependent induction H; auto.
-      cbn in x0; dependent destruction x0.
-      apply H1; eauto.
-      exact Fin.F1.
-    - now apply AFIndBase.
+    induction n; intros.
+    - specialize (H Fin.F1).
+      dependent induction H.
+      + (* AFIndNow *) now left.
+      + (* AFIndDone *)
+        right; intros.
+        dependent destruction i; try solve [inv i].
+        split; unfold can_step; cbn; rewrite H.
+        * exists Ctree.stuck, (Done x).
+          now econstructor.
+        * intros * TR.
+          dependent destruction TR.
+          now apply AFNowIndBase.
+      + (* AFIndFinish *)
+        right; intros.
+        dependent destruction i; try solve [inv i].
+        split; unfold can_step; cbn; rewrite H.
+        * exists Ctree.stuck, (Finish e v x).
+          now econstructor.
+        * intros * TR.
+          dependent destruction TR.
+          now apply AFNowIndBase.
+      + (* AFIndBr *) destruct b.
+        * (* BrS *) right.
+          intro i.
+          dependent destruction i; try solve [inv i].
+          unfold can_step; cbn; setoid_rewrite H.
+          split; intros.
+          -- exists (k0 Fin.F1), w; try econstructor; auto.
+          -- admit. 
+        * (* BrD *)
+          induction n.
+          -- edestruct H2.
+  Admitted.
+
+  Lemma pull1_iff: forall {A B} (P : A -> Prop) (R : A -> B -> Prop),
+      (forall a, (exists b, R a b)-> P a) <-> (forall a b, R a b -> P a).
+    split; intros; eauto.
+    destruct H0.
+    now apply H with x.
   Qed.
 
+  Lemma pull2_iff: forall {A B C} (P : A -> B -> Prop) (R : A -> B -> C -> Prop),
+      (forall a b, (exists c, R a b c)-> P a b) <-> (forall a b c, R a b c -> P a b).
+    split; intros; eauto.
+    destruct H0.
+    now apply H with x.
+  Qed.
+    
   (* This is a super useful lemma, it allows us to do
      induction on [AFInd] instead of two inductions on
      [cau] and [trans] *)
   Opaque Ctree.stuck.
-  Lemma af_afind : forall (t: ctree E X) (w: World E),
-       cau true (fun _ _ => True) φ t w -> AFInd t w.
-  Proof.
-    intros; induction H.
-    - now apply AFIndBase.
+  Lemma af_afind : forall (t: ctree E X) (w: World E) φ,
+       <( t, w |= AF now φ )> -> AFNowInd φ t w.
+  Proof.    
+    intros; cbn in H.
+    induction H.
+    - now apply AFNowIndBase.
     - destruct H0, H1; clear H H1.
-      destruct H0 as (t' & w' & TR).
-      cbn in TR.
-      
-      (* induction on ktrans_ for ctrees *)      
-      dependent induction TR.
-      + (* BrD *)
-        eapply AFIndBr; eauto.
-        intro i'.        
-        eapply H3; cbn.
-        rewrite <- x0.
-        apply KtransBrD with i'.
-
-        
-        eapply IHTR. with t'; auto.
-      + eapply AFIndVis with (e:=e); auto.
-        observe_equ x.
-        
-        intros v'.
-        apply H3; cbn.
-        rewrite <- x0.
-        apply KtransObs; auto.
-      + eapply AFIndTau with (u:=t0); auto.
-        eapply (IHTR) with (t':=t'); auto.
-        -- intros t_ w_ TR_.
-           apply H2; cbn.
-           rewrite <- x0.
-           now apply ktrans_tau.
-        -- intros t_ w_ TR_.
-           apply H3; cbn.
-           rewrite <- x0.
-           now apply ktrans_tau.
-      + apply AFIndDoneBase with (x:=x0); auto.
-        assert (TR_: [t, Pure] ↦ [Ctree.stuck, Done x0]).
-        { cbn; rewrite <- x1; apply KtransDone; auto. }
-        specialize (H3 _ _ TR_).
-        now apply af_ind_stuck_done.
-      + apply AFIndFinishBase with (x:=x0); auto.
-        assert (TR_: [t, Obs e v] ↦ [Ctree.stuck, Finish e v x0]).
-        { cbn; rewrite <- x1; apply KtransFinish; auto. }
-        specialize (H3 _ _ TR_).
-        now apply af_ind_stuck_finish.
-  Qed.
+      destruct H0 as (t' & w' & TR).      
+      cbn in TR; desobs t. 
+      + (* RetF *)
+        destruct w; cbn in H2, H3; setoid_rewrite Heqt in H2;
+          setoid_rewrite Heqt in H3.
+        * (* RetF, Pure *)
+          destruct (H2 _ _ TR); dependent destruction TR.
+          -- apply AFNowIndDone with x0; auto.
+          -- destruct H1.
+             apply can_step_not_done in H1.
+             inv H1.
+        * (* RetF, Obs e v *)
+          destruct (H2 _ _ TR); dependent destruction TR.
+          -- apply AFNowIndFinish with x0; auto.
+          -- destruct H1.
+             apply can_step_not_done in H1.
+             inv H1.
+        * (* RetF, Done *) dependent destruction TR.
+        * (* RetF, Finish *) dependent destruction TR.
+      + (* Br b n k *)
+        apply AFNowIndBr with b n k; auto.
+        * apply ktrans_not_done with (Br b n k) t' w'; auto.
+        * destruct b.
+          -- (* BrS *)
+            intros i Hs.
+            apply ktrans_brS in TR as (? & ? & -> & ?).
+            apply H3; cbn.
+            rewrite Heqt.
+            apply ktrans_brS.
+            exists i; auto.
+          -- (* BrD *)
+            intros i (t_ & w_ & TR_).
+            assert(TR': [t, w] ↦ [t_, w_]).
+            { cbn; rewrite Heqt; apply ktrans_brD; exists i; auto. }
+            cbn in TR_, TR', H2, H3.
+            rewrite Heqt in *.
+            clear TR TR_ t' w'.
+            specialize (H2 t_ w_ TR').
+            specialize (H3 t_ w_ TR').            
+            clear t Heqt.
+            rewrite ctree_eta.
+            rewrite ctree_eta in H2, H3.
+            remember (BrF false n k) as T.
+            remember (observe t_) as T_.            
+            clear HeqT_ t_.
+            revert i.
+            generalize dependent n.
+            generalize dependent φ.
+            dependent induction TR'; intros; dependent destruction HeqT.
+            apply AFNowIndBr with false n0 k0;  eauto.            
+            (* BrD *)            
+            ++ cbn. admit.
+            ++ now apply ktrans_not_done with (k0 i) t' w'.
+            ++ intros j Hs.
+               rewrite ctree_eta.
+               apply IHTR'; auto.
+               admit.
+      + (* Vis e k *)
+        apply AFNowIndVis with e k; auto.
+        * apply ktrans_not_done with (Vis e k) t' w'; auto.
+        * intros v. 
+          apply ktrans_vis in TR as (? & -> & ? & ?).
+          apply H3; cbn.
+          rewrite Heqt.
+          apply ktrans_vis.
+          exists v; auto.
+  Admitted.
   
-  (* -> *)
-  Lemma afind_af {Hpr: @Productive E HE}
-    {HP: Proper (equ X ==> eq ==> iff) φ}
-    {TauInv: forall (t: ctree E X) w, φ t w  -> φ (Tau t) w}
-    : forall (t: ctree E X) (w: World E),
-      AFInd t w -> cau true (fun _ _ => True) φ t w.
-  Proof.
-    intros; induction H.
-    - now apply MatchA.
-    - apply StepA; auto; split.
-      + exists Ctree.stuck, (Done x).
-        Opaque Ctree.stuck.
-        cbn. rewrite H.
-        apply KtransDone; auto.
-      + intros t' w' TR.
-        ktrans_ind TR.
-        * rewrite H in x1; inv x1.
-        * rewrite H in x1; inv x1.
-        * rewrite H in x2; inv x2.          
-          observe_equ x.
-          rewrite <- Eqt, H1.          
-          now apply MatchA.
-    - apply StepA; auto; split.
-      + exists Ctree.stuck, (Finish e v x).
-        Opaque Ctree.stuck.
-        cbn. rewrite H.
-        apply KtransFinish; auto.
-      + intros t' w' TR.
-        ktrans_ind TR.
-        * rewrite H in x1; inv x1.
-        * rewrite H in x1; inv x1.
-        * rewrite H in x2; inv x2.          
-          observe_equ x.
-          rewrite <- Eqt, H1.          
-          now apply MatchA.
-    - observe_equ H.
-      rewrite Eqt; clear Eqt.
-      destruct IHAFInd.
-      + apply MatchA.
-        (* TauInv here *)
-        now apply TauInv.
-      + destruct H2.
-        apply StepA; auto.
-        split; auto with ctl.
-        intros t' w' TR.
-        apply H3.
-        now rewrite ktrans_tau in TR.
-    - observe_equ H.
-      rewrite Eqt; clear Eqt.
-      apply StepA; auto; split; auto with ctl.
-      intros t' w' TR.
-      + apply ktrans_vis in TR as (v & ? & -> & ?).
-        rewrite H3.
-        eapply H2.
-  Qed.
 End AfIndLemma.
